pKVM-simplified-model/extraction/extraction.v
@@ -30,5 +30,5 @@ Set Extraction Flag 2031.
 Set Extraction Output Directory ".".
 
 Extraction "coq_executable_sm.ml"
-  all_steps state_0 step_
+  all_steps memory_0 step
   state_fold zallocd_fold.
